# B2

## Problem

Let $f:[0,1] \to [0,\infty)$ be strictly increasing and continuous. Let $R$ be the region bounded by $x = 0$, $x = 1$, $y = 0$, and $y = f(x)$.

Let $x_1$ be the $x$-coordinate of the centroid of $R$. Let $x_2$ be the $x$-coordinate of the **centroid of the solid** generated by rotating $R$ about the $x$-axis.

Prove that $x_1 < x_2$.

## Submission

To prove that $ x_1 < x_2 $, we analyze the centroids of two different geometric objects derived from a strictly increasing and continuous function $ f: [0,1] \to [0,\infty) $.

---

### **Step 1: Definitions**

Let $ R $ be the region bounded by $ x = 0 $, $ x = 1 $, $ y = 0 $, and $ y = f(x) $. The **centroid** of this region has an $ x $-coordinate given by:

$$
x_1 = \frac{\int_0^1 x f(x) \, dx}{\int_0^1 f(x) \, dx}
$$

Now consider the solid formed by rotating $ R $ about the $ x $-axis. This solid is symmetric about the $ x $-axis, so its centroid lies on the axis of rotation. The $ x $-coordinate of the centroid of the solid is:

$$
x_2 = \frac{\int_0^1 x f(x)^2 \, dx}{\int_0^1 f(x)^2 \, dx}
$$

Our goal is to show that $ x_1 < x_2 $.

---

### **Step 2: Reformulate the Inequality**

We aim to show:
$$
x_1 < x_2 \quad \Leftrightarrow \quad \frac{\int_0^1 x f(x) \, dx}{\int_0^1 f(x) \, dx} < \frac{\int_0^1 x f(x)^2 \, dx}{\int_0^1 f(x)^2 \, dx}
$$

Cross-multiplying (since all integrals are positive due to $ f $ being strictly increasing and continuous on $[0,1]$), we get the equivalent inequality:

$$
\left( \int_0^1 x f(x) \, dx \right) \left( \int_0^1 f(x)^2 \, dx \right) < \left( \int_0^1 x f(x)^2 \, dx \right) \left( \int_0^1 f(x) \, dx \right)
$$

Let us define:
- $ N_1 = \int_0^1 x f(x) \, dx $
- $ D_1 = \int_0^1 f(x) \, dx $
- $ N_2 = \int_0^1 x f(x)^2 \, dx $
- $ D_2 = \int_0^1 f(x)^2 \, dx $

Then the desired inequality becomes:
$$
N_1 D_2 < N_2 D_1
$$

This is equivalent to:
$$
N_2 D_1 - N_1 D_2 > 0
$$

---

### **Step 3: Use of Strict Monotonicity**

Let $ T = x_1 = \frac{N_1}{D_1} $. Then,
$$
N_2 D_1 - N_1 D_2 = D_1 \left( N_2 - T D_2 \right) = D_1 \int_0^1 (x - T) f(x)^2 \, dx
$$

So,
$$
x_2 - x_1 = \frac{N_2 - T D_2}{D_2} = \frac{1}{D_2} \int_0^1 (x - T) f(x)^2 \, dx
$$

Thus, it suffices to show that:
$$
\int_0^1 (x - T) f(x)^2 \, dx > 0
$$

---

### **Step 4: Analyze the Integrand**

Define:
$$
g(x) = (x - T) f(x)^2
$$

Note that:
$$
g(x) = (x - T) f(x)^2 = (x - T) f(x) \cdot f(x)
$$

Let’s examine the sign of $ g(x) $ using the fact that $ f $ is **strictly increasing**.

For any $ x \neq T $, since $ f $ is strictly increasing:
- If $ x > T $, then $ f(x) > f(T) $, so $ (x - T) > 0 $ and $ f(x) - f(T) > 0 $, hence $ (x - T)(f(x) - f(T)) > 0 $
- If $ x < T $, then $ f(x) < f(T) $, so $ (x - T) < 0 $ and $ f(x) - f(T) < 0 $, hence $ (x - T)(f(x) - f(T)) > 0 $

Therefore, for all $ x \neq T $, we have:
$$
(x - T)(f(x) - f(T)) > 0
$$

Now observe:
$$
(x - T)f(x)^2 = (x - T)f(x) \cdot f(x) = (x - T)f(T) \cdot f(x) + (x - T)(f(x) - f(T))f(x)
$$

But $ \int_0^1 (x - T)f(x) \, dx = 0 $ by definition of $ T $, so:
$$
\int_0^1 (x - T)f(x)^2 \, dx = \int_0^1 (x - T)(f(x) - f(T))f(x) \, dx
$$

The integrand $ (x - T)(f(x) - f(T))f(x) $ is **non-negative everywhere**, and **positive almost everywhere** (except at $ x = T $, which has measure zero). Therefore, the integral is **strictly positive**.

---

### **Conclusion**

Since $ x_2 - x_1 = \frac{1}{D_2} \int_0^1 (x - T)f(x)^2 \, dx > 0 $, we conclude:

$$
x_1 < x_2
$$

This holds for all strictly increasing and continuous functions $ f: [0,1] \to [0,\infty) $, as required.

---

### ✅ Final Answer:

$$
\boxed{x_1 < x_2}
$$
