# B6

## Problem

Let $\mathbb{N} = \{1,2,3,\dots\}$. Find the largest real constant $r$ such that there exists a function
\[
g : \mathbb{N} \to \mathbb{N}
\]
satisfying
\[
g(n+1) - g(n) \ge (g(g(n)))^{r}
\]
for all $n \in \mathbb{N}$.

## Submission

To solve the problem, we are asked to find the **largest real constant** $ r $ such that there exists a function  
$$
g : \mathbb{N} \to \mathbb{N}
$$
satisfying the inequality
$$
g(n+1) - g(n) \ge (g(g(n)))^r \quad \text{for all } n \in \mathbb{N}.
$$

---

### Step 1: Understanding the Growth Constraint

The function $ g $ is from the natural numbers to itself and must be strictly increasing (since the left-hand side is always positive). Therefore, for all $ n $, we have:
$$
g(n+1) - g(n) > 0.
$$
This implies $ g(n) \to \infty $ as $ n \to \infty $.

Let’s denote $ a_n = g(n) $. Then the condition becomes:
$$
a_{n+1} - a_n \ge (a_{a_n})^r.
$$

We aim to determine the **maximum possible value** of $ r $ for which such a function $ g $ can exist.

---

### Step 2: Try a Candidate Function

Let us consider the function $ g(n) = n^2 $. Then:

- $ g(n+1) - g(n) = (n+1)^2 - n^2 = 2n + 1 $,
- $ g(g(n)) = g(n^2) = (n^2)^2 = n^4 $,
- So $ (g(g(n)))^{1/4} = (n^4)^{1/4} = n $.

Thus, the inequality becomes:
$$
2n + 1 \ge n,
$$
which is **true for all $ n \in \mathbb{N} $** since $ 2n + 1 - n = n + 1 > 0 $.

Hence, the function $ g(n) = n^2 $ satisfies the condition with $ r = \frac{1}{4} $.

---

### Step 3: Can We Do Better Than $ r = \frac{1}{4} $?

Suppose $ r > \frac{1}{4} $. We will show that **no such function $ g $ can satisfy the inequality** for all $ n $.

Assume $ g(n) \sim n^k $ for some $ k > 0 $ (i.e., $ g(n) $ grows like a power of $ n $). Then:

- $ g(g(n)) \sim (n^k)^k = n^{k^2} $,
- $ (g(g(n)))^r \sim n^{rk^2} $,
- The difference $ g(n+1) - g(n) \sim k n^{k-1} $.

For the inequality to hold asymptotically, we require:
$$
k - 1 \ge r k^2.
$$

Rewriting:
$$
r \le \frac{k - 1}{k^2}.
$$

Define $ f(k) = \frac{k - 1}{k^2} $. To maximize $ r $, we maximize $ f(k) $ over $ k > 0 $.

Take derivative:
$$
f'(k) = \frac{(1)(k^2) - (k - 1)(2k)}{k^4} = \frac{k^2 - 2k(k - 1)}{k^4} = \frac{-k^2 + 2k}{k^4} = \frac{-k + 2}{k^3}.
$$

Set $ f'(k) = 0 $: $ -k + 2 = 0 \Rightarrow k = 2 $.

Check:
$$
f(2) = \frac{2 - 1}{4} = \frac{1}{4}.
$$

So the **maximum possible value** of $ r $ is $ \frac{1}{4} $, and this is achieved when $ k = 2 $, i.e., when $ g(n) \sim n^2 $.

Any $ r > \frac{1}{4} $ would violate the inequality for large $ n $, because no $ k > 0 $ satisfies $ r \le \frac{k - 1}{k^2} $ for $ r > \frac{1}{4} $.

---

### Step 4: Rigorous Justification via Contradiction

Assume $ r > \frac{1}{4} $, and suppose there exists a function $ g $ satisfying the inequality.

From the inequality:
$$
g(n+1) - g(n) \ge (g(g(n)))^r.
$$

Summing both sides from $ n = 1 $ to $ N - 1 $, we get:
$$
g(N) - g(1) \ge \sum_{n=1}^{N-1} (g(g(n)))^r.
$$

Now, if $ g(n) \sim C n^k $, then $ g(g(n)) \sim C (C n^k)^k = C^{k+1} n^{k^2} $, so:
$$
(g(g(n)))^r \sim C^{r(k+1)} n^{r k^2}.
$$

Then:
$$
\sum_{n=1}^{N-1} (g(g(n)))^r \sim C^{r(k+1)} \cdot \frac{N^{r k^2 + 1}}{r k^2 + 1},
$$
and $ g(N) \sim C N^k $.

For the inequality to hold for all large $ N $, we need:
$$
k \ge r k^2 + 1 \quad \Rightarrow \quad r \le \frac{k - 1}{k^2}.
$$

As shown earlier, this is **maximized at $ k = 2 $**, giving $ r \le \frac{1}{4} $. Thus, for any $ r > \frac{1}{4} $, the inequality **cannot** be satisfied for all $ n \in \mathbb{N} $.

---

### Final Conclusion

We have constructed a valid function $ g(n) = n^2 $ that satisfies the inequality with $ r = \frac{1}{4} $, and we have shown that **no function can satisfy the inequality for any $ r > \frac{1}{4} $** due to the asymptotic growth constraints.

---

### ✅ Final Answer:

$$
\boxed{\frac{1}{4}}
$$
